cedar-lean/Cedar/Thm/Validation/Typechecker/And.lean
@@ -26,71 +26,73 @@ open Cedar.Data
 open Cedar.Spec
 open Cedar.Validation
 
-theorem type_of_and_inversion {x₁ x₂ : Expr} {c c' : Capabilities} {env : Environment} {ty : CedarType}
+theorem type_of_and_inversion {x₁ x₂ : Expr} {c c' : Capabilities} {env : Environment} {ty : TypedExpr}
   (h₁ : typeOf (Expr.and x₁ x₂) c env = Except.ok (ty, c')) :
   ∃ bty₁ c₁,
-    typeOf x₁ c env = .ok (.bool bty₁, c₁) ∧
+    (typeOf x₁ c env).typeOf = .ok (.bool bty₁, c₁) ∧
     if bty₁ = BoolType.ff
-    then ty = .bool BoolType.ff ∧ c' = ∅
+    then ty.typeOf = .bool BoolType.ff ∧ c' = ∅
     else ∃ bty₂ c₂,
-      typeOf x₂ (c ∪ c₁) env = .ok (.bool bty₂, c₂) ∧
+      (typeOf x₂ (c ∪ c₁) env).typeOf = .ok (.bool bty₂, c₂) ∧
       if bty₂ = BoolType.ff
-      then ty = .bool BoolType.ff ∧ c' = ∅
-      else ty = .bool (lubBool bty₁ bty₂) ∧ c' = c₁ ∪ c₂
+      then ty.typeOf = .bool BoolType.ff ∧ c' = ∅
+      else ty.typeOf = .bool (lubBool bty₁ bty₂) ∧ c' = c₁ ∪ c₂
 := by
   simp [typeOf] at h₁
   cases h₂ : typeOf x₁ c env <;> simp [h₂] at *
   rename_i res₁
-  simp [typeOfAnd] at h₁
+  simp only [typeOfAnd, List.empty_eq] at h₁
   split at h₁ <;> simp [ok, err] at h₁
   case ok.h_1 h₃ =>
-    exists BoolType.ff, res₁.snd ; simp [h₁]
-    simp at h₃
-    have ⟨h₁, _⟩ := h₁ ; subst h₁
-    have ⟨h₃, _⟩ := h₃
-    simp [←h₃]
+    have ⟨ hl₁, hr₁ ⟩ := h₁
+    subst hl₁ hr₁
+    exists BoolType.ff, res₁.snd
+    simp only [Prod.mk.injEq] at h₃
+    simp [ResultType.typeOf, Except.map, h₃]
   case ok.h_2 bty₁ c₁ h₃ h₄ =>
     exists bty₁, c₁
     simp at h₄
     have ⟨hty₁, hc₁⟩ := h₄
-    simp [←hty₁, ←hc₁]
+    simp [←hty₁, ←hc₁, ResultType.typeOf, Except.map]
     split ; contradiction
     cases h₄ : typeOf x₂ (c ∪ res₁.snd) env <;> simp [h₄] at *
     rename_i res₂
     split at h₁ <;> simp at h₁ <;>
     have ⟨hty, hc⟩ := h₁ <;> subst hty hc
     case isFalse.ok.h_1 hty₂ =>
-      exists BoolType.ff, res₂.snd ; simp [←hty₂]
+      exists BoolType.ff, res₂.snd
     case isFalse.ok.h_2 hty₂ =>
       exists BoolType.tt, res₂.snd ; simp [←hty₂, hc₁]
-      cases bty₁ <;> simp at h₃ <;> simp [lubBool]
+      cases bty₁ <;> simp at h₃ <;> simp [lubBool, TypedExpr.typeOf]
     case isFalse.ok.h_3 bty₂ h₄ h₅ hty₂ =>
       exists BoolType.anyBool, res₂.snd
       cases bty₂ <;> simp at *
-      simp [←hty₂, hc₁, lubBool]
+      simp [hty₂, hc₁, lubBool]
       split <;> rename_i h₆
-      · simp [h₆]
+      · simp [h₆, TypedExpr.typeOf]
       · rfl
 
-theorem type_of_and_is_sound {x₁ x₂ : Expr} {c₁ c₂ : Capabilities} {env : Environment} {ty : CedarType} {request : Request} {entities : Entities}
+theorem type_of_and_is_sound {x₁ x₂ : Expr} {c₁ c₂ : Capabilities} {env : Environment} {ty : TypedExpr} {request : Request} {entities : Entities}
   (h₁ : CapabilitiesInvariant c₁ request entities)
   (h₂ : RequestAndEntitiesMatchEnvironment env request entities)
   (h₃ : typeOf (Expr.and x₁ x₂) c₁ env = Except.ok (ty, c₂))
   (ih₁ : TypeOfIsSound x₁)
   (ih₂ : TypeOfIsSound x₂) :
   GuardedCapabilitiesInvariant (Expr.and x₁ x₂) c₂ request entities ∧
-  ∃ v, EvaluatesTo (Expr.and x₁ x₂) request entities v ∧ InstanceOfType v ty
+  ∃ v, EvaluatesTo (Expr.and x₁ x₂) request entities v ∧ InstanceOfType v ty.typeOf
 := by
   have ⟨bty₁, rc₁, h₄, h₅⟩ := type_of_and_inversion h₃
-  specialize ih₁ h₁ h₂ h₄
+  split_type_of h₄ ; rename_i h'₄ hl₄ hr₄
+  specialize ih₁ h₁ h₂ h'₄
   have ⟨ih₁₁, v₁, ih₁₂, ih₁₃⟩ := ih₁
+  rw [hl₄] at ih₁₃
   have ⟨b₁, hb₁⟩ := instance_of_bool_is_bool ih₁₃
   subst hb₁
   split at h₅
   case isTrue h₆ =>
     subst h₆
     have ⟨hty, hc⟩ := h₅
-    subst hty hc
+    rw [hty, hc]
     apply And.intro empty_guarded_capabilities_invariant
     have h₇ := instance_of_ff_is_false ih₁₃
     simp at h₇ ; subst h₇
@@ -101,7 +103,7 @@ theorem type_of_and_is_sound {x₁ x₂ : Expr} {c₁ c₂ : Capabilities} {env 
     exact false_is_instance_of_ff
   case isFalse h₆ =>
     have ⟨bty₂, rc₂, hₜ, h₇⟩ := h₅
-    split at h₇ <;> have ⟨hty, hc⟩ := h₇ <;> subst hty hc
+    split at h₇ <;> have ⟨hty, hc⟩ := h₇ <;> rw [hty, hc]
     case isTrue h₈ =>
       subst h₈
       apply And.intro empty_guarded_capabilities_invariant
@@ -116,11 +118,14 @@ theorem type_of_and_is_sound {x₁ x₂ : Expr} {c₁ c₂ : Capabilities} {env 
         simp [GuardedCapabilitiesInvariant] at ih₁₁
         specialize ih₁₁ ih₁₂
         have h₇ := capability_union_invariant h₁ ih₁₁
-        specialize ih₂ h₇ h₂ hₜ
+        split_type_of hₜ ; rename_i h'ₜ hlₜ hrₜ
+        subst hr₄
+        specialize ih₂ h₇ h₂ h'ₜ
         have ⟨_, v₂, ih₂₂, ih₂₃⟩ := ih₂
         simp [EvaluatesTo] at ih₂₂
         rcases ih₂₂ with ih₂₂ | ih₂₂ | ih₂₂ | ih₂₂ <;>
         simp [Result.as, ih₂₂, Coe.coe, Value.asBool, Lean.Internal.coeM, pure, Except.pure]
+        rw [hlₜ] at ih₂₃
         have h₈ := instance_of_ff_is_false ih₂₃
         subst h₈
         simp [CoeT.coe, CoeHTCT.coe, CoeHTC.coe, CoeOTC.coe, CoeTC.coe, Coe.coe]
@@ -138,13 +143,16 @@ theorem type_of_and_is_sound {x₁ x₂ : Expr} {c₁ c₂ : Capabilities} {env 
         try exact type_is_inhabited (CedarType.bool (lubBool bty₁ bty₂))
         simp [GuardedCapabilitiesInvariant] at ih₁₁
         specialize ih₁₁ ih₁₂
+        split_type_of hₜ ; rename_i h'ₜ hlₜ hrₜ
+        subst hr₄
         have h₇ := capability_union_invariant h₁ ih₁₁
-        specialize ih₂ h₇ h₂ hₜ
+        specialize ih₂ h₇ h₂ h'ₜ
         have ⟨ih₂₁, v₂, ih₂₂, ih₂₃⟩ := ih₂
         simp [EvaluatesTo] at ih₂₂
         rcases ih₂₂ with ih₂₂ | ih₂₂ | ih₂₂ | ih₂₂ <;>
         simp [EvaluatesTo, evaluate, Result.as, ih₂₂, Coe.coe, Value.asBool, Lean.Internal.coeM, pure, Except.pure] <;>
         try exact type_is_inhabited (CedarType.bool (lubBool bty₁ bty₂))
+        rw [hlₜ] at ih₂₃
         have ⟨b₂, hb₂⟩ := instance_of_bool_is_bool ih₂₃
         subst hb₂
         cases b₂ <;> simp [CoeT.coe, CoeHTCT.coe, CoeHTC.coe, CoeOTC.coe, CoeTC.coe, Coe.coe]
@@ -154,6 +162,7 @@ theorem type_of_and_is_sound {x₁ x₂ : Expr} {c₁ c₂ : Capabilities} {env 
           apply And.intro
           · simp [GuardedCapabilitiesInvariant] at ih₂₁
             specialize ih₂₁ ih₂₂
+            rw [hrₜ] at ih₂₁
             exact capability_union_invariant ih₁₁ ih₂₁
           · apply instance_of_lubBool ; simp [ih₁₃]
 
